<?xml version="1.0"?>


<!DOCTYPE rdf:RDF [
    <!ENTITY owl "http://www.w3.org/2002/07/owl#" >
    <!ENTITY mpeg7x "http://metadata.net/mpeg7/mpeg7x#" >
    <!ENTITY xsd "http://www.w3.org/2001/XMLSchema#" >
    <!ENTITY mpeg7 "http://metadata.net/mpeg7/mpeg7.owl#" >
    <!ENTITY rdfs "http://www.w3.org/2000/01/rdf-schema#" >
    <!ENTITY rdf "http://www.w3.org/1999/02/22-rdf-syntax-ns#" >
]>


<rdf:RDF xmlns="http://metadata.net/mpeg7/mpeg7x#"
     xml:base="http://metadata.net/mpeg7/mpeg7x"
     xmlns:mpeg7="http://metadata.net/mpeg7/mpeg7.owl#"
     xmlns:rdfs="http://www.w3.org/2000/01/rdf-schema#"
     xmlns:owl="http://www.w3.org/2002/07/owl#"
     xmlns:xsd="http://www.w3.org/2001/XMLSchema#"
     xmlns:rdf="http://www.w3.org/1999/02/22-rdf-syntax-ns#"
     xmlns:mpeg7x="http://metadata.net/mpeg7/mpeg7x#">
    <owl:Ontology rdf:about="">
        <rdfs:label>MPEG-7 extensions</rdfs:label>
        <owl:versionInfo>v 1.0 2006/11/06 12:56:51 slittle</owl:versionInfo>
        <rdfs:comment>Extensions to the MPEG-7 ontology (http://metadata.net/mpeg7) to
			incorporate image analysis terms including some from MATLAB.</rdfs:comment>
        <owl:imports rdf:resource="http://metadata.net/mpeg7/mpeg7.owl"/>
    </owl:Ontology>
    


    <!-- 
    ///////////////////////////////////////////////////////////////////////////////////////
    //
    // Annotation properties
    //
    ///////////////////////////////////////////////////////////////////////////////////////
     -->

    <owl:AnnotationProperty rdf:about="&owl;versionInfo"/>
    <owl:AnnotationProperty rdf:about="&rdfs;label"/>
    <owl:AnnotationProperty rdf:about="&rdfs;comment"/>
    


    <!-- 
    ///////////////////////////////////////////////////////////////////////////////////////
    //
    // Object Properties
    //
    ///////////////////////////////////////////////////////////////////////////////////////
     -->

    


    <!-- http://metadata.net/mpeg7/mpeg7.owl#color -->

    <owl:ObjectProperty rdf:about="&mpeg7;color"/>
    


    <!-- http://metadata.net/mpeg7/mpeg7x#colorRange -->

    <owl:ObjectProperty rdf:about="#colorRange">
        <rdfs:label>color range</rdfs:label>
        <rdfs:comment>Lightest color minus darkest color in a region</rdfs:comment>
        <rdfs:subPropertyOf rdf:resource="&mpeg7;color"/>
    </owl:ObjectProperty>
    


    <!-- http://metadata.net/mpeg7/mpeg7x#colorVariation -->

    <owl:ObjectProperty rdf:about="#colorVariation">
        <rdfs:label>color variation</rdfs:label>
        <rdfs:comment>standard deviation of the set of colors in a region</rdfs:comment>
        <rdfs:subPropertyOf rdf:resource="&mpeg7;color"/>
    </owl:ObjectProperty>
    


    <!-- http://metadata.net/mpeg7/mpeg7x#darkestColor -->

    <owl:ObjectProperty rdf:about="#darkestColor">
        <rdfs:label>darkest color</rdfs:label>
        <rdfs:comment>min of the set of colors in a region</rdfs:comment>
        <rdfs:subPropertyOf rdf:resource="&mpeg7;color"/>
    </owl:ObjectProperty>
    


    <!-- http://metadata.net/mpeg7/mpeg7x#dominantColorRange -->

    <owl:ObjectProperty rdf:about="#dominantColorRange">
        <rdfs:label>dominant color range</rdfs:label>
        <rdfs:comment>The range of colors (increments of 10 from Darkest to Lightest color) that is most common</rdfs:comment>
        <rdfs:subPropertyOf rdf:resource="&mpeg7;color"/>
    </owl:ObjectProperty>
    


    <!-- http://metadata.net/mpeg7/mpeg7x#lightestColor -->

    <owl:ObjectProperty rdf:about="#lightestColor">
        <rdfs:label>lightest color</rdfs:label>
        <rdfs:comment>max of the set of colors in a region</rdfs:comment>
        <rdfs:subPropertyOf rdf:resource="&mpeg7;color"/>
    </owl:ObjectProperty>
    


    <!-- http://metadata.net/mpeg7/mpeg7x#meanColor -->

    <owl:ObjectProperty rdf:about="#meanColor">
        <rdfs:label>mean color</rdfs:label>
        <rdfs:comment>mean or average of the set of colors in a region</rdfs:comment>
        <rdfs:subPropertyOf rdf:resource="&mpeg7;color"/>
    </owl:ObjectProperty>
    


    <!-- 
    ///////////////////////////////////////////////////////////////////////////////////////
    //
    // Data properties
    //
    ///////////////////////////////////////////////////////////////////////////////////////
     -->

    


    <!-- http://metadata.net/mpeg7/mpeg7x#area -->

    <owl:DatatypeProperty rdf:about="#area">
        <rdfs:label>area</rdfs:label>
        <rdfs:comment>Area of the region, usually measured in number of pixels</rdfs:comment>
        <rdfs:subPropertyOf rdf:resource="#matlabVisualFeature"/>
    </owl:DatatypeProperty>
    


    <!-- http://metadata.net/mpeg7/mpeg7x#convexArea -->

    <owl:DatatypeProperty rdf:about="#convexArea">
        <rdfs:label>convex area</rdfs:label>
        <rdfs:comment>the number of pixels in the convex image - the smallest convex polygon that can contain the region</rdfs:comment>
        <rdfs:subPropertyOf rdf:resource="#matlabVisualFeature"/>
    </owl:DatatypeProperty>
    


    <!-- http://metadata.net/mpeg7/mpeg7x#eccentricity -->

    <owl:DatatypeProperty rdf:about="#eccentricity">
        <rdfs:label>eccentricity</rdfs:label>
        <rdfs:comment>the ratio of the distance between the foci of the ellipse and its major axis length</rdfs:comment>
        <rdfs:subPropertyOf rdf:resource="#matlabVisualFeature"/>
    </owl:DatatypeProperty>
    


    <!-- http://metadata.net/mpeg7/mpeg7x#equivDiameter -->

    <owl:DatatypeProperty rdf:about="#equivDiameter">
        <rdfs:label>equivalent diameter</rdfs:label>
        <rdfs:comment>the diameter of a circle with the same area as the region. Computed as sqrt(4*Area/pi)</rdfs:comment>
        <rdfs:subPropertyOf rdf:resource="#matlabVisualFeature"/>
    </owl:DatatypeProperty>
    


    <!-- http://metadata.net/mpeg7/mpeg7x#eulerNumber -->

    <owl:DatatypeProperty rdf:about="#eulerNumber">
        <rdfs:label>euler number</rdfs:label>
        <rdfs:comment>equal to the number of objects in the region minus the number of holes in those objects</rdfs:comment>
        <rdfs:subPropertyOf rdf:resource="#matlabVisualFeature"/>
    </owl:DatatypeProperty>
    


    <!-- http://metadata.net/mpeg7/mpeg7x#extent -->

    <owl:DatatypeProperty rdf:about="#extent">
        <rdfs:label>extent</rdfs:label>
        <rdfs:comment>the proportion of the pixels in the bounding box that are also in the region. Computed as the Area divided by the area of the bounding box</rdfs:comment>
        <rdfs:subPropertyOf rdf:resource="#matlabVisualFeature"/>
    </owl:DatatypeProperty>
    


    <!-- http://metadata.net/mpeg7/mpeg7x#filledArea -->

    <owl:DatatypeProperty rdf:about="#filledArea">
        <rdfs:label>filled area</rdfs:label>
        <rdfs:comment>the number of &#39;on&#39; pixels in the filled image</rdfs:comment>
        <rdfs:subPropertyOf rdf:resource="#matlabVisualFeature"/>
    </owl:DatatypeProperty>
    


    <!-- http://metadata.net/mpeg7/mpeg7x#majorAxisLength -->

    <owl:DatatypeProperty rdf:about="#majorAxisLength">
        <rdfs:label>major axis length</rdfs:label>
        <rdfs:comment>the length (in pixels) of the major axis of the ellipse that has the same normalized second central moments as the region</rdfs:comment>
        <rdfs:subPropertyOf rdf:resource="#matlabVisualFeature"/>
    </owl:DatatypeProperty>
    


    <!-- http://metadata.net/mpeg7/mpeg7x#matlabVisualFeature -->

    <owl:DatatypeProperty rdf:about="#matlabVisualFeature">
        <rdfs:label>MatlabVisualFeature</rdfs:label>
        <rdfs:comment>Image analysis measurements produced by the MATLAB Image Analysis Toolbox</rdfs:comment>
        <rdfs:domain rdf:resource="&mpeg7;StillRegion"/>
        <rdfs:range rdf:resource="&xsd;decimal"/>
    </owl:DatatypeProperty>
    


    <!-- http://metadata.net/mpeg7/mpeg7x#minorAxisLength -->

    <owl:DatatypeProperty rdf:about="#minorAxisLength">
        <rdfs:label>minor axis length</rdfs:label>
        <rdfs:comment>the length (in pixels) of the minor axis of the ellipse that has the same normalized second central moments as the region</rdfs:comment>
        <rdfs:subPropertyOf rdf:resource="#matlabVisualFeature"/>
    </owl:DatatypeProperty>
    


    <!-- http://metadata.net/mpeg7/mpeg7x#orientation -->

    <owl:DatatypeProperty rdf:about="#orientation">
        <rdfs:label>orientation</rdfs:label>
        <rdfs:comment>the angle (in degrees) between the x-axis and the major axis of the ellipse</rdfs:comment>
        <rdfs:subPropertyOf rdf:resource="#matlabVisualFeature"/>
    </owl:DatatypeProperty>
    


    <!-- http://metadata.net/mpeg7/mpeg7x#solidity -->

    <owl:DatatypeProperty rdf:about="#solidity">
        <rdfs:label>solidity</rdfs:label>
        <rdfs:comment>the proportion of the pixels in the convex hull that are also in the region. Computed as Area/ConvexArea</rdfs:comment>
        <rdfs:subPropertyOf rdf:resource="#matlabVisualFeature"/>
    </owl:DatatypeProperty>
    


    <!-- 
    ///////////////////////////////////////////////////////////////////////////////////////
    //
    // Classes
    //
    ///////////////////////////////////////////////////////////////////////////////////////
     -->

    


    <!-- http://metadata.net/mpeg7/mpeg7.owl#StillRegion -->

    <owl:Class rdf:about="&mpeg7;StillRegion"/>
</rdf:RDF>



<!-- Generated by the OWL API (version 3.0.0) http://owlapi.sourceforge.net -->

